<?xml version="1.0"?>
<rdf:RDF xmlns="https://purl.org/andreapoltronieri/scorepart/"
     xml:base="https://purl.org/andreapoltronieri/scorepart/"
     xmlns:dc="http://purl.org/dc/elements/1.1/"
     xmlns:owl="http://www.w3.org/2002/07/owl#"
     xmlns:rdf="http://www.w3.org/1999/02/22-rdf-syntax-ns#"
     xmlns:xml="http://www.w3.org/XML/1998/namespace"
     xmlns:xsd="http://www.w3.org/2001/XMLSchema#"
     xmlns:opla="http://ontologydesignpatterns.org/opla/"
     xmlns:rdfs="http://www.w3.org/2000/01/rdf-schema#"
     xmlns:terms="http://purl.org/dc/terms/"
     xmlns:cpannotationschema="http://www.ontologydesignpatterns.org/schemas/cpannotationschema.owl#">
    <owl:Ontology rdf:about="https://purl.org/andreapoltronieri/scorepart/">
        <dc:creator rdf:datatype="http://www.w3.org/2001/XMLSchema#string">Andrea Poltronieri (University of Bologna)</dc:creator>
        <dc:description xml:lang="en">The Score Part module models the structure and the hierarchies of a music score.</dc:description>
        <dc:language rdf:resource="http://publications.europa.eu/resource/authority/language/ENG"/>
        <dc:title xml:lang="en">Score Part Pattern</dc:title>
        <terms:issued>2021-07-17</terms:issued>
        <terms:license rdf:resource="https://creativecommons.org/licenses/by-sa/4.0/"/>
        <cpannotationschema:coversRequirements xml:lang="en">What is the instrument playing a specific score part?, How many voices does the score part have?, Which are the metrics defining the sections of the score part?</cpannotationschema:coversRequirements>
        <cpannotationschema:extractedFrom rdf:resource="https://purl.org/andreapoltronieri/notepattern"/>
        <cpannotationschema:hasComponent rdf:resource="http://ontologydesignpatterns.org/wiki/Submissions:PartOf"/>
        <cpannotationschema:hasIntent xml:lang="en">This content ODP formalises the structure and the hierarchies of a music score/symbolic representation system.</cpannotationschema:hasIntent>
        <cpannotationschema:reengineeredFrom rdf:resource="https://purl.org/andreapoltronieri/HaMSEontology"/>
        <rdfs:comment xml:lang="en">The Score Part pattern models the structure and the hierarchies of a music score.
In this module are used as template the following Ontology Design Patterns:</rdfs:comment>
        <rdfs:label xml:lang="en">Score Part Pattern</rdfs:label>
        <owl:versionInfo xml:lang="en">Version 1.0</owl:versionInfo>
    </owl:Ontology>
    


    <!-- 
    ///////////////////////////////////////////////////////////////////////////////////////
    //
    // Annotation properties
    //
    ///////////////////////////////////////////////////////////////////////////////////////
     -->

    


    <!-- http://ontologydesignpatterns.org/opla/reusesPatternAsTemplate -->

    <owl:AnnotationProperty rdf:about="http://ontologydesignpatterns.org/opla/reusesPatternAsTemplate"/>
    


    <!-- http://purl.org/dc/elements/1.1/creator -->

    <owl:AnnotationProperty rdf:about="http://purl.org/dc/elements/1.1/creator"/>
    


    <!-- http://purl.org/dc/elements/1.1/description -->

    <owl:AnnotationProperty rdf:about="http://purl.org/dc/elements/1.1/description"/>
    


    <!-- http://purl.org/dc/elements/1.1/language -->

    <owl:AnnotationProperty rdf:about="http://purl.org/dc/elements/1.1/language"/>
    


    <!-- http://purl.org/dc/elements/1.1/title -->

    <owl:AnnotationProperty rdf:about="http://purl.org/dc/elements/1.1/title"/>
    


    <!-- http://purl.org/dc/terms/issued -->

    <owl:AnnotationProperty rdf:about="http://purl.org/dc/terms/issued"/>
    


    <!-- http://purl.org/dc/terms/license -->

    <owl:AnnotationProperty rdf:about="http://purl.org/dc/terms/license"/>
    


    <!-- http://www.ontologydesignpatterns.org/schemas/cpannotationschema.owl#coversRequirements -->

    <owl:AnnotationProperty rdf:about="http://www.ontologydesignpatterns.org/schemas/cpannotationschema.owl#coversRequirements">
        <rdfs:comment>This annotation property is used for exemplifying possible requirements the content pattern provides a solution for. Requirements are expressed as natural language competency questions.</rdfs:comment>
    </owl:AnnotationProperty>
    


    <!-- http://www.ontologydesignpatterns.org/schemas/cpannotationschema.owl#extractedFrom -->

    <owl:AnnotationProperty rdf:about="http://www.ontologydesignpatterns.org/schemas/cpannotationschema.owl#extractedFrom">
        <rdfs:comment>This annotation property should be assigned with a URI, which points to the possible reference ontology which the annotated pattern was extracted from (i.e. the reference ontology that the ontology elements have been deeply or partially cloned by). The range is not explicit in the definition of the annotation property because it would turn the ontology to OWL Full. E.g. The participation pattern is extracted from the Dolce Ultra Lite ontology, hence the value for this annotation property is http://www.ontologydesignpatterns.org/ont/dul/DUL.owl</rdfs:comment>
    </owl:AnnotationProperty>
    


    <!-- http://www.ontologydesignpatterns.org/schemas/cpannotationschema.owl#hasComponent -->

    <owl:AnnotationProperty rdf:about="http://www.ontologydesignpatterns.org/schemas/cpannotationschema.owl#hasComponent">
        <rdfs:comment>This annotation property is useful for content ontology design patterns. Its value is a URI, which refers to another content ontology design pattern which is a component of the annotated one.</rdfs:comment>
    </owl:AnnotationProperty>
    


    <!-- http://www.ontologydesignpatterns.org/schemas/cpannotationschema.owl#hasConsequences -->

    <owl:AnnotationProperty rdf:about="http://www.ontologydesignpatterns.org/schemas/cpannotationschema.owl#hasConsequences">
        <rdfs:comment>This annotation property is used for briefly describing the benefits and/or possible trade-offs when using the CP.</rdfs:comment>
    </owl:AnnotationProperty>
    


    <!-- http://www.ontologydesignpatterns.org/schemas/cpannotationschema.owl#hasIntent -->

    <owl:AnnotationProperty rdf:about="http://www.ontologydesignpatterns.org/schemas/cpannotationschema.owl#hasIntent">
        <rdfs:comment>This annotation property is used in order to describe the intent of the content pattern.</rdfs:comment>
    </owl:AnnotationProperty>
    


    <!-- http://www.ontologydesignpatterns.org/schemas/cpannotationschema.owl#hasUnitTest -->

    <owl:AnnotationProperty rdf:about="http://www.ontologydesignpatterns.org/schemas/cpannotationschema.owl#hasUnitTest">
        <rdfs:comment>This property can be used to annotate a unit test (e.g. in the form of a SPARQL query) to be launched to evaluate an ontology against a requirement-based task.</rdfs:comment>
    </owl:AnnotationProperty>
    


    <!-- http://www.ontologydesignpatterns.org/schemas/cpannotationschema.owl#isCloneOf -->

    <owl:AnnotationProperty rdf:about="http://www.ontologydesignpatterns.org/schemas/cpannotationschema.owl#isCloneOf">
        <rdfs:comment>This annotation property is used for referring a cloned ontology entity to its cloning source.</rdfs:comment>
    </owl:AnnotationProperty>
    


    <!-- http://www.ontologydesignpatterns.org/schemas/cpannotationschema.owl#isSpecializationOf -->

    <owl:AnnotationProperty rdf:about="http://www.ontologydesignpatterns.org/schemas/cpannotationschema.owl#isSpecializationOf">
        <rdfs:comment>This annotation property is useful for content ontology design patterns and its elements. Its value is a URI, which refers either to a content ontology design pattern that is specialized by the annotated one, or to an ontology element that is specialized by the annotated one.</rdfs:comment>
    </owl:AnnotationProperty>
    


    <!-- http://www.ontologydesignpatterns.org/schemas/cpannotationschema.owl#reengineeredFrom -->

    <owl:AnnotationProperty rdf:about="http://www.ontologydesignpatterns.org/schemas/cpannotationschema.owl#reengineeredFrom">
        <rdfs:comment>This annotation property should be assigned with a URI, which points to the concept schema, page, or anything else from which the annotated pattern was reengineered. If the source does not have any URI e.g., a printed book, this property value should provide information as precise as possible in order to identify the source. This property is alternative to the extractedFrom property because it is used when the pattern come from a concept schema which is not an owl ontology. For example content ontology design patterns, which are reengineered from data model patterns, rdf schemas, etc. should be annotatd with this property. E.g. The basicpersonalfoaf pattern is extracted from the rdf FOAF specification, hence the value for this annotation property is http://xmlns.com/foaf/spec/20071002.rdf</rdfs:comment>
    </owl:AnnotationProperty>
    


    <!-- http://www.ontologydesignpatterns.org/schemas/cpannotationschema.owl#relatedCPs -->

    <owl:AnnotationProperty rdf:about="http://www.ontologydesignpatterns.org/schemas/cpannotationschema.owl#relatedCPs">
        <rdfs:comment>This annotation property can be used to indicate other CPs (if any) that specialize, generalize, inlcude, or are components of the CP. Furthermore, this field may indicate other CPs that are typically used in conjunction with the described one. Important similarities and differences with other patterns can be also described here.</rdfs:comment>
    </owl:AnnotationProperty>
    


    <!-- http://www.ontologydesignpatterns.org/schemas/cpannotationschema.owl#scenarios -->

    <owl:AnnotationProperty rdf:about="http://www.ontologydesignpatterns.org/schemas/cpannotationschema.owl#scenarios">
        <rdfs:comment>This annotation property is used for describing examples of instantiation of the Content OP. For example, for the part-of Content OP (which represents part-whole relations) a possible scenario is the sentence: &quot;the brain is part of the human body&quot;. Scenarios are expressed as natural language sentences.</rdfs:comment>
    </owl:AnnotationProperty>
    


    <!-- http://www.w3.org/2002/07/owl#versionInfo -->

    <owl:AnnotationProperty rdf:about="http://www.w3.org/2002/07/owl#versionInfo"/>
    


    <!-- 
    ///////////////////////////////////////////////////////////////////////////////////////
    //
    // Object Properties
    //
    ///////////////////////////////////////////////////////////////////////////////////////
     -->

    


    <!-- https://purl.org/andreapoltronieri/scorepart/hasFragment -->

    <owl:ObjectProperty rdf:about="https://purl.org/andreapoltronieri/scorepart/hasFragment">
        <owl:inverseOf rdf:resource="https://purl.org/andreapoltronieri/scorepart/isFragmentOf"/>
        <rdfs:domain rdf:resource="https://purl.org/andreapoltronieri/scorepart/Part"/>
        <rdfs:range rdf:resource="https://purl.org/andreapoltronieri/scorepart/HomogeneousFragment"/>
        <rdfs:comment xml:lang="en">Connects the part of the score/symbolic notation to its constituing sections.</rdfs:comment>
        <rdfs:label xml:lang="en">has section</rdfs:label>
    </owl:ObjectProperty>
    


    <!-- https://purl.org/andreapoltronieri/scorepart/hasSection -->

    <owl:ObjectProperty rdf:about="https://purl.org/andreapoltronieri/scorepart/hasSection">
        <owl:inverseOf rdf:resource="https://purl.org/andreapoltronieri/scorepart/isSectionOf"/>
        <rdfs:domain rdf:resource="https://purl.org/andreapoltronieri/scorepart/Part"/>
        <rdfs:range rdf:resource="https://purl.org/andreapoltronieri/scorepart/Section"/>
        <rdfs:label xml:lang="en">has section</rdfs:label>
    </owl:ObjectProperty>
    


    <!-- https://purl.org/andreapoltronieri/scorepart/hasVoice -->

    <owl:ObjectProperty rdf:about="https://purl.org/andreapoltronieri/scorepart/hasVoice">
        <owl:inverseOf rdf:resource="https://purl.org/andreapoltronieri/scorepart/isVoiceOf"/>
        <rdf:type rdf:resource="http://www.w3.org/2002/07/owl#InverseFunctionalProperty"/>
        <rdfs:domain rdf:resource="https://purl.org/andreapoltronieri/scorepart/Part"/>
        <rdfs:range rdf:resource="https://purl.org/andreapoltronieri/scorepart/Voice"/>
        <rdfs:comment xml:lang="en">Connects the part of the score/symbolic notation to its constituing sections.</rdfs:comment>
        <rdfs:label xml:lang="en">has voice</rdfs:label>
    </owl:ObjectProperty>
    


    <!-- https://purl.org/andreapoltronieri/scorepart/isFragmentOf -->

    <owl:ObjectProperty rdf:about="https://purl.org/andreapoltronieri/scorepart/isFragmentOf">
        <rdfs:domain rdf:resource="https://purl.org/andreapoltronieri/scorepart/HomogeneousFragment"/>
        <rdfs:range rdf:resource="https://purl.org/andreapoltronieri/scorepart/Part"/>
        <rdfs:comment xml:lang="en">Inverse of hasFragment. Connects the section of the score/symbolic notation to the belongng part.</rdfs:comment>
        <rdfs:label xml:lang="en">is section of</rdfs:label>
    </owl:ObjectProperty>
    


    <!-- https://purl.org/andreapoltronieri/scorepart/isPlayedBy -->

    <owl:ObjectProperty rdf:about="https://purl.org/andreapoltronieri/scorepart/isPlayedBy">
        <owl:inverseOf rdf:resource="https://purl.org/andreapoltronieri/scorepart/playsPart"/>
        <rdfs:domain rdf:resource="https://purl.org/andreapoltronieri/scorepart/Part"/>
        <rdfs:range rdf:resource="https://purl.org/andreapoltronieri/scorepart/Instrument"/>
        <rdfs:comment xml:lang="en">Connects the part of the score/symbolic notation to the instrument that is assigned to play such part.</rdfs:comment>
        <rdfs:label xml:lang="en">is played by</rdfs:label>
    </owl:ObjectProperty>
    


    <!-- https://purl.org/andreapoltronieri/scorepart/isSectionOf -->

    <owl:ObjectProperty rdf:about="https://purl.org/andreapoltronieri/scorepart/isSectionOf">
        <rdfs:domain rdf:resource="https://purl.org/andreapoltronieri/scorepart/Section"/>
        <rdfs:range rdf:resource="https://purl.org/andreapoltronieri/scorepart/Part"/>
        <rdfs:label xml:lang="en">is section of</rdfs:label>
    </owl:ObjectProperty>
    


    <!-- https://purl.org/andreapoltronieri/scorepart/isVoiceOf -->

    <owl:ObjectProperty rdf:about="https://purl.org/andreapoltronieri/scorepart/isVoiceOf">
        <rdf:type rdf:resource="http://www.w3.org/2002/07/owl#FunctionalProperty"/>
        <rdfs:domain rdf:resource="https://purl.org/andreapoltronieri/scorepart/Voice"/>
        <rdfs:range rdf:resource="https://purl.org/andreapoltronieri/scorepart/Part"/>
        <rdfs:comment xml:lang="en">Inverse of hasVoice. Connects the voice of the score/symbolic notation to the belongng part.</rdfs:comment>
        <rdfs:label xml:lang="en">is voice of</rdfs:label>
    </owl:ObjectProperty>
    


    <!-- https://purl.org/andreapoltronieri/scorepart/playsPart -->

    <owl:ObjectProperty rdf:about="https://purl.org/andreapoltronieri/scorepart/playsPart">
        <rdfs:domain rdf:resource="https://purl.org/andreapoltronieri/scorepart/Instrument"/>
        <rdfs:range rdf:resource="https://purl.org/andreapoltronieri/scorepart/Part"/>
        <rdfs:comment xml:lang="en">Inverse of isPlayedBy. Connects an instrument to the the part that the instrument plays.</rdfs:comment>
        <rdfs:label xml:lang="en">plays part</rdfs:label>
    </owl:ObjectProperty>
    


    <!-- 
    ///////////////////////////////////////////////////////////////////////////////////////
    //
    // Data properties
    //
    ///////////////////////////////////////////////////////////////////////////////////////
     -->

    


    <!-- https://purl.org/andreapoltronieri/scorepart/hasClef -->

    <owl:DatatypeProperty rdf:about="https://purl.org/andreapoltronieri/scorepart/hasClef">
        <rdf:type rdf:resource="http://www.w3.org/2002/07/owl#FunctionalProperty"/>
        <rdfs:domain rdf:resource="https://purl.org/andreapoltronieri/scorepart/HomogeneousFragment"/>
        <rdfs:range rdf:resource="http://www.w3.org/2001/XMLSchema#string"/>
        <rdfs:comment xml:lang="en">The clef that describes the hight of a note in a music score fragment.</rdfs:comment>
        <rdfs:label xml:lang="en">has clef</rdfs:label>
    </owl:DatatypeProperty>
    


    <!-- https://purl.org/andreapoltronieri/scorepart/hasMetric -->

    <owl:DatatypeProperty rdf:about="https://purl.org/andreapoltronieri/scorepart/hasMetric">
        <rdf:type rdf:resource="http://www.w3.org/2002/07/owl#FunctionalProperty"/>
        <rdfs:domain rdf:resource="https://purl.org/andreapoltronieri/scorepart/HomogeneousFragment"/>
        <rdfs:range rdf:resource="http://www.w3.org/2001/XMLSchema#int"/>
        <rdfs:comment xml:lang="en">The metric of a specific fragment of a music score.</rdfs:comment>
        <rdfs:label xml:lang="en">has metric</rdfs:label>
    </owl:DatatypeProperty>
    


    <!-- https://purl.org/andreapoltronieri/scorepart/hasMidiProgram -->

    <owl:DatatypeProperty rdf:about="https://purl.org/andreapoltronieri/scorepart/hasMidiProgram">
        <rdf:type rdf:resource="http://www.w3.org/2002/07/owl#FunctionalProperty"/>
        <rdfs:domain rdf:resource="https://purl.org/andreapoltronieri/scorepart/Instrument"/>
        <rdfs:range rdf:resource="http://www.w3.org/2001/XMLSchema#int"/>
        <rdfs:comment xml:lang="en">The instrument playing a specific part expressed by a MIDI program.</rdfs:comment>
        <rdfs:label xml:lang="en">has midi program</rdfs:label>
    </owl:DatatypeProperty>
    


    <!-- https://purl.org/andreapoltronieri/scorepart/hasStaff -->

    <owl:DatatypeProperty rdf:about="https://purl.org/andreapoltronieri/scorepart/hasStaff">
        <rdf:type rdf:resource="http://www.w3.org/2002/07/owl#FunctionalProperty"/>
        <rdfs:domain rdf:resource="https://purl.org/andreapoltronieri/scorepart/Part"/>
        <rdfs:range rdf:resource="http://www.w3.org/2000/01/rdf-schema#Literal"/>
        <rdfs:comment xml:lang="en">The staff assigned to a specific instrument part in a music score.</rdfs:comment>
        <rdfs:label xml:lang="en">has staff</rdfs:label>
    </owl:DatatypeProperty>
    


    <!-- https://purl.org/andreapoltronieri/scorepart/hasTempo -->

    <owl:DatatypeProperty rdf:about="https://purl.org/andreapoltronieri/scorepart/hasTempo">
        <rdf:type rdf:resource="http://www.w3.org/2002/07/owl#FunctionalProperty"/>
        <rdfs:domain rdf:resource="https://purl.org/andreapoltronieri/scorepart/HomogeneousFragment"/>
        <rdfs:range rdf:resource="http://www.w3.org/2001/XMLSchema#int"/>
        <rdfs:comment xml:lang="en">The tempo of an homogeneous fragment, expressed in bpm (integer).</rdfs:comment>
        <rdfs:label xml:lang="en">has tempo</rdfs:label>
    </owl:DatatypeProperty>
    


    <!-- 
    ///////////////////////////////////////////////////////////////////////////////////////
    //
    // Classes
    //
    ///////////////////////////////////////////////////////////////////////////////////////
     -->

    


    <!-- https://purl.org/andreapoltronieri/scorepart/HomogeneousFragment -->

    <owl:Class rdf:about="https://purl.org/andreapoltronieri/scorepart/HomogeneousFragment">
        <owl:equivalentClass>
            <owl:Class>
                <owl:intersectionOf rdf:parseType="Collection">
                    <rdf:Description rdf:about="https://purl.org/andreapoltronieri/scorepart/Part"/>
                    <owl:Restriction>
                        <owl:onProperty rdf:resource="https://purl.org/andreapoltronieri/scorepart/hasFragment"/>
                        <owl:cardinality rdf:datatype="http://www.w3.org/2001/XMLSchema#nonNegativeInteger">1</owl:cardinality>
                    </owl:Restriction>
                </owl:intersectionOf>
            </owl:Class>
        </owl:equivalentClass>
        <rdfs:subClassOf>
            <owl:Restriction>
                <owl:onProperty rdf:resource="https://purl.org/andreapoltronieri/scorepart/isFragmentOf"/>
                <owl:allValuesFrom rdf:resource="https://purl.org/andreapoltronieri/scorepart/Part"/>
            </owl:Restriction>
        </rdfs:subClassOf>
        <rdfs:subClassOf>
            <owl:Restriction>
                <owl:onProperty rdf:resource="https://purl.org/andreapoltronieri/scorepart/hasClef"/>
                <owl:qualifiedCardinality rdf:datatype="http://www.w3.org/2001/XMLSchema#nonNegativeInteger">1</owl:qualifiedCardinality>
                <owl:onDataRange rdf:resource="http://www.w3.org/2001/XMLSchema#string"/>
            </owl:Restriction>
        </rdfs:subClassOf>
        <rdfs:subClassOf>
            <owl:Restriction>
                <owl:onProperty rdf:resource="https://purl.org/andreapoltronieri/scorepart/hasMetric"/>
                <owl:qualifiedCardinality rdf:datatype="http://www.w3.org/2001/XMLSchema#nonNegativeInteger">1</owl:qualifiedCardinality>
                <owl:onDataRange rdf:resource="http://www.w3.org/2001/XMLSchema#int"/>
            </owl:Restriction>
        </rdfs:subClassOf>
        <rdfs:subClassOf>
            <owl:Restriction>
                <owl:onProperty rdf:resource="https://purl.org/andreapoltronieri/scorepart/hasTempo"/>
                <owl:qualifiedCardinality rdf:datatype="http://www.w3.org/2001/XMLSchema#nonNegativeInteger">1</owl:qualifiedCardinality>
                <owl:onDataRange rdf:resource="http://www.w3.org/2001/XMLSchema#int"/>
            </owl:Restriction>
        </rdfs:subClassOf>
        <owl:disjointWith rdf:resource="https://purl.org/andreapoltronieri/scorepart/Instrument"/>
        <rdfs:comment xml:lang="en">A group of notes that share the same metric and clef.</rdfs:comment>
        <rdfs:label xml:lang="en">Section</rdfs:label>
    </owl:Class>
    


    <!-- https://purl.org/andreapoltronieri/scorepart/Instrument -->

    <owl:Class rdf:about="https://purl.org/andreapoltronieri/scorepart/Instrument">
        <rdfs:subClassOf>
            <owl:Restriction>
                <owl:onProperty rdf:resource="https://purl.org/andreapoltronieri/scorepart/playsPart"/>
                <owl:someValuesFrom rdf:resource="https://purl.org/andreapoltronieri/scorepart/Part"/>
            </owl:Restriction>
        </rdfs:subClassOf>
        <owl:disjointWith rdf:resource="https://purl.org/andreapoltronieri/scorepart/Section"/>
        <owl:disjointWith rdf:resource="https://purl.org/andreapoltronieri/scorepart/Voice"/>
        <rdfs:comment xml:lang="en">Any of various devices or contrivances that can be used to produce musical tones or sound. Any taxonomy can be used to subsume this concept. The default one is one extracted by Ivan Herman from the Musicbrainz instrument taxonomy, conforming to SKOS. This concept holds a seeAlso link towards this taxonomy.</rdfs:comment>
        <rdfs:label xml:lang="en">Instrument</rdfs:label>
    </owl:Class>
    


    <!-- https://purl.org/andreapoltronieri/scorepart/Part -->

    <owl:Class rdf:about="https://purl.org/andreapoltronieri/scorepart/Part">
        <rdfs:subClassOf>
            <owl:Restriction>
                <owl:onProperty rdf:resource="https://purl.org/andreapoltronieri/scorepart/hasFragment"/>
                <owl:minQualifiedCardinality rdf:datatype="http://www.w3.org/2001/XMLSchema#nonNegativeInteger">1</owl:minQualifiedCardinality>
                <owl:onClass rdf:resource="https://purl.org/andreapoltronieri/scorepart/HomogeneousFragment"/>
            </owl:Restriction>
        </rdfs:subClassOf>
        <rdfs:subClassOf>
            <owl:Restriction>
                <owl:onProperty rdf:resource="https://purl.org/andreapoltronieri/scorepart/hasSection"/>
                <owl:minQualifiedCardinality rdf:datatype="http://www.w3.org/2001/XMLSchema#nonNegativeInteger">1</owl:minQualifiedCardinality>
                <owl:onClass rdf:resource="https://purl.org/andreapoltronieri/scorepart/Section"/>
            </owl:Restriction>
        </rdfs:subClassOf>
        <rdfs:subClassOf>
            <owl:Restriction>
                <owl:onProperty rdf:resource="https://purl.org/andreapoltronieri/scorepart/hasVoice"/>
                <owl:minQualifiedCardinality rdf:datatype="http://www.w3.org/2001/XMLSchema#nonNegativeInteger">1</owl:minQualifiedCardinality>
                <owl:onClass rdf:resource="https://purl.org/andreapoltronieri/scorepart/Voice"/>
            </owl:Restriction>
        </rdfs:subClassOf>
        <rdfs:subClassOf>
            <owl:Restriction>
                <owl:onProperty rdf:resource="https://purl.org/andreapoltronieri/scorepart/isPlayedBy"/>
                <owl:minQualifiedCardinality rdf:datatype="http://www.w3.org/2001/XMLSchema#nonNegativeInteger">1</owl:minQualifiedCardinality>
                <owl:onClass rdf:resource="https://purl.org/andreapoltronieri/scorepart/Instrument"/>
            </owl:Restriction>
        </rdfs:subClassOf>
        <rdfs:subClassOf>
            <owl:Restriction>
                <owl:onProperty rdf:resource="https://purl.org/andreapoltronieri/scorepart/hasStaff"/>
                <owl:qualifiedCardinality rdf:datatype="http://www.w3.org/2001/XMLSchema#nonNegativeInteger">1</owl:qualifiedCardinality>
                <owl:onDataRange rdf:resource="http://www.w3.org/2001/XMLSchema#int"/>
            </owl:Restriction>
        </rdfs:subClassOf>
        <rdfs:comment xml:lang="en">A part of a a score notation or a symbolic notation assigned to a specific instrument.</rdfs:comment>
        <rdfs:label xml:lang="en">Part</rdfs:label>
    </owl:Class>
    


    <!-- https://purl.org/andreapoltronieri/scorepart/Section -->

    <owl:Class rdf:about="https://purl.org/andreapoltronieri/scorepart/Section">
        <owl:equivalentClass>
            <owl:Class>
                <owl:intersectionOf rdf:parseType="Collection">
                    <rdf:Description rdf:about="https://purl.org/andreapoltronieri/scorepart/Part"/>
                    <owl:Restriction>
                        <owl:onProperty rdf:resource="https://purl.org/andreapoltronieri/scorepart/hasSection"/>
                        <owl:qualifiedCardinality rdf:datatype="http://www.w3.org/2001/XMLSchema#nonNegativeInteger">1</owl:qualifiedCardinality>
                        <owl:onClass rdf:resource="https://purl.org/andreapoltronieri/scorepart/Section"/>
                    </owl:Restriction>
                </owl:intersectionOf>
            </owl:Class>
        </owl:equivalentClass>
        <rdfs:subClassOf>
            <owl:Restriction>
                <owl:onProperty rdf:resource="https://purl.org/andreapoltronieri/scorepart/isSectionOf"/>
                <owl:qualifiedCardinality rdf:datatype="http://www.w3.org/2001/XMLSchema#nonNegativeInteger">1</owl:qualifiedCardinality>
                <owl:onClass rdf:resource="https://purl.org/andreapoltronieri/scorepart/Part"/>
            </owl:Restriction>
        </rdfs:subClassOf>
        <rdfs:comment xml:lang="en">A section as defined by the repetition signs found on the music score.</rdfs:comment>
        <rdfs:label xml:lang="en">Section</rdfs:label>
    </owl:Class>
    


    <!-- https://purl.org/andreapoltronieri/scorepart/Voice -->

    <owl:Class rdf:about="https://purl.org/andreapoltronieri/scorepart/Voice">
        <owl:equivalentClass>
            <owl:Class>
                <owl:intersectionOf rdf:parseType="Collection">
                    <rdf:Description rdf:about="https://purl.org/andreapoltronieri/scorepart/Part"/>
                    <owl:Restriction>
                        <owl:onProperty rdf:resource="https://purl.org/andreapoltronieri/scorepart/hasVoice"/>
                        <owl:cardinality rdf:datatype="http://www.w3.org/2001/XMLSchema#nonNegativeInteger">1</owl:cardinality>
                    </owl:Restriction>
                </owl:intersectionOf>
            </owl:Class>
        </owl:equivalentClass>
        <rdfs:subClassOf>
            <owl:Restriction>
                <owl:onProperty rdf:resource="https://purl.org/andreapoltronieri/scorepart/isVoiceOf"/>
                <owl:allValuesFrom rdf:resource="https://purl.org/andreapoltronieri/scorepart/Part"/>
            </owl:Restriction>
        </rdfs:subClassOf>
        <rdfs:comment xml:lang="en">One of several parts that can be performed within the same staff (e.g. alto and soprano).</rdfs:comment>
        <rdfs:label xml:lang="en">Voice</rdfs:label>
    </owl:Class>
</rdf:RDF>



<!-- Generated by the OWL API (version 4.5.9.2019-02-01T07:24:44Z) https://github.com/owlcs/owlapi -->

