<?xml version="1.0"?>
<rdf:RDF xmlns="https://w3id.org/polifonia/ontology/music-representation/"
     xml:base="https://w3id.org/polifonia/ontology/music-representation/"
     xmlns:dc="http://purl.org/dc/elements/1.1/"
     xmlns:mso="http://linkeddata.uni-muenster.de/ontology/musicscore#"
     xmlns:mto="http://purl.org/ontology/mto/"
     xmlns:owl="http://www.w3.org/2002/07/owl#"
     xmlns:rdf="http://www.w3.org/1999/02/22-rdf-syntax-ns#"
     xmlns:xml="http://www.w3.org/XML/1998/namespace"
     xmlns:xsd="http://www.w3.org/2001/XMLSchema#"
     xmlns:core="https://w3id.org/polifonia/ontology/core/"
     xmlns:meta="https://w3id.org/polifonia/ontology/music-meta/"
     xmlns:rdfs="http://www.w3.org/2000/01/rdf-schema#"
     xmlns:skos="http://www.w3.org/2004/02/skos/core#"
     xmlns:terms="http://purl.org/dc/terms/"
     xmlns:explanation="http://linkedu.eu/dedalo/explanationPattern.owl#"
     xmlns:cpannotationschema="http://www.ontologydesignpatterns.org/schemas/cpannotationschema.owl#">
    <owl:Ontology rdf:about="https://w3id.org/polifonia/ontology/music-representation/">
        <owl:imports rdf:resource="http://linkeddata.uni-muenster.de/ontology/musicscore#1.0.0"/>
        <owl:imports rdf:resource="http://linkedu.eu/dedalo/explanationPattern.owl"/>
        <owl:imports rdf:resource="http://www.ontologydesignpatterns.org/cp/owl/descriptionandsituation.owl"/>
        <owl:imports rdf:resource="http://www.ontologydesignpatterns.org/cp/owl/informationrealization.owl"/>
        <owl:imports rdf:resource="http://www.ontologydesignpatterns.org/cp/owl/partof.owl"/>
        <owl:imports rdf:resource="http://www.w3.org/2004/02/skos/core"/>
        <owl:imports rdf:resource="https://w3id.org/polifonia/ontology/core/0.1/"/>
        <owl:imports rdf:resource="https://w3id.org/polifonia/ontology/music-meta/1.0/"/>
    </owl:Ontology>
    


    <!-- 
    ///////////////////////////////////////////////////////////////////////////////////////
    //
    // Object Properties
    //
    ///////////////////////////////////////////////////////////////////////////////////////
     -->

    


    <!-- https://w3id.org/polifonia/ontology/music-representation/derivesFrom -->

    <owl:ObjectProperty rdf:about="https://w3id.org/polifonia/ontology/music-representation/derivesFrom">
        <rdf:type rdf:resource="http://www.w3.org/2002/07/owl#TransitiveProperty"/>
        <rdfs:comment xml:lang="en">Relationship between two annotation. Defines the dependency that the first annotation has on the second one.</rdfs:comment>
        <rdfs:label xml:lang="en">derives from</rdfs:label>
    </owl:ObjectProperty>
    


    <!-- https://w3id.org/polifonia/ontology/music-representation/describes -->

    <owl:ObjectProperty rdf:about="https://w3id.org/polifonia/ontology/music-representation/describes">
        <rdfs:subPropertyOf rdf:resource="http://www.ontologydesignpatterns.org/cp/owl/descriptionandsituation.owl#describes"/>
        <rdfs:domain rdf:resource="https://w3id.org/polifonia/ontology/music-representation/Annotation"/>
        <rdfs:range rdf:resource="https://w3id.org/polifonia/ontology/music-representation/Fragment"/>
        <rdfs:comment xml:lang="en">The relation between an annotation and the fragment it is describing.</rdfs:comment>
        <rdfs:label xml:lang="en">describes</rdfs:label>
    </owl:ObjectProperty>
    


    <!-- https://w3id.org/polifonia/ontology/music-representation/hasAnnotationContent -->

    <owl:ObjectProperty rdf:about="https://w3id.org/polifonia/ontology/music-representation/hasAnnotationContent">
        <rdf:type rdf:resource="http://www.w3.org/2002/07/owl#FunctionalProperty"/>
        <rdf:type rdf:resource="http://www.w3.org/2002/07/owl#InverseFunctionalProperty"/>
        <rdfs:domain rdf:resource="https://w3id.org/polifonia/ontology/music-representation/Annotation"/>
        <rdfs:range rdf:resource="https://w3id.org/polifonia/ontology/music-representation/AnnotationContent"/>
        <rdfs:comment xml:lang="en">The relation between an annotation and its content.</rdfs:comment>
        <rdfs:label xml:lang="en">has annotation content</rdfs:label>
    </owl:ObjectProperty>
    


    <!-- https://w3id.org/polifonia/ontology/music-representation/hasAnnotationType -->

    <owl:ObjectProperty rdf:about="https://w3id.org/polifonia/ontology/music-representation/hasAnnotationType">
        <rdf:type rdf:resource="http://www.w3.org/2002/07/owl#FunctionalProperty"/>
        <rdfs:domain rdf:resource="https://w3id.org/polifonia/ontology/music-representation/Annotation"/>
        <rdfs:range rdf:resource="https://w3id.org/polifonia/ontology/music-representation/AnnotationType"/>
        <rdfs:comment xml:lang="en">The relationship that defines the type of an annotation.</rdfs:comment>
        <rdfs:label xml:lang="en">has annotation type</rdfs:label>
    </owl:ObjectProperty>
    


    <!-- https://w3id.org/polifonia/ontology/music-representation/hasAnnotator -->

    <owl:ObjectProperty rdf:about="https://w3id.org/polifonia/ontology/music-representation/hasAnnotator">
        <rdfs:domain rdf:resource="https://w3id.org/polifonia/ontology/music-representation/Annotation"/>
        <rdfs:range rdf:resource="https://w3id.org/polifonia/ontology/core/Agent"/>
        <rdfs:comment xml:lang="en">The relationship that identifies an agent that contributed to an annotation.</rdfs:comment>
        <rdfs:label xml:lang="en">has annotator</rdfs:label>
    </owl:ObjectProperty>
    


    <!-- https://w3id.org/polifonia/ontology/music-representation/hasAnnotatorType -->

    <owl:ObjectProperty rdf:about="https://w3id.org/polifonia/ontology/music-representation/hasAnnotatorType">
        <rdf:type rdf:resource="http://www.w3.org/2002/07/owl#FunctionalProperty"/>
        <rdfs:domain rdf:resource="https://w3id.org/polifonia/ontology/core/Agent"/>
        <rdfs:range rdf:resource="https://w3id.org/polifonia/ontology/music-representation/AnnotatorType"/>
        <rdfs:comment xml:lang="en">The type of an annotator (e.g. domain expert)</rdfs:comment>
        <rdfs:label xml:lang="en">has annotator type</rdfs:label>
    </owl:ObjectProperty>
    


    <!-- https://w3id.org/polifonia/ontology/music-representation/hasFeatures -->

    <owl:ObjectProperty rdf:about="https://w3id.org/polifonia/ontology/music-representation/hasFeatures">
        <rdfs:domain rdf:resource="https://w3id.org/polifonia/ontology/music-meta/Recording"/>
        <rdfs:range rdf:resource="https://w3id.org/polifonia/ontology/music-representation/AudioFeatures"/>
    </owl:ObjectProperty>
    


    <!-- https://w3id.org/polifonia/ontology/music-representation/hasFragment -->

    <owl:ObjectProperty rdf:about="https://w3id.org/polifonia/ontology/music-representation/hasFragment">
        <rdfs:subPropertyOf rdf:resource="http://www.ontologydesignpatterns.org/cp/owl/partof.owl#hasPart"/>
        <rdfs:domain rdf:resource="https://w3id.org/polifonia/ontology/music-representation/MusicContent"/>
        <rdfs:range rdf:resource="https://w3id.org/polifonia/ontology/music-representation/Fragment"/>
        <rdfs:comment xml:lang="en">The relation that connects an atomic fragment to the corresponding music content.</rdfs:comment>
        <rdfs:label xml:lang="en">has fragment</rdfs:label>
    </owl:ObjectProperty>
    


    <!-- https://w3id.org/polifonia/ontology/music-representation/hasSubject -->

    <owl:ObjectProperty rdf:about="https://w3id.org/polifonia/ontology/music-representation/hasSubject">
        <rdfs:subPropertyOf rdf:resource="http://www.ontologydesignpatterns.org/cp/owl/informationrealization.owl#realizes"/>
        <rdfs:domain rdf:resource="https://w3id.org/polifonia/ontology/music-representation/AnnotationContent"/>
        <rdfs:range rdf:resource="https://w3id.org/polifonia/ontology/music-representation/MusicNotation"/>
        <rdfs:comment xml:lang="en">The relation that identifies a subject of interest in an annotation content.</rdfs:comment>
        <rdfs:label xml:lang="en">has subject</rdfs:label>
    </owl:ObjectProperty>
    


    <!-- https://w3id.org/polifonia/ontology/music-representation/isAnalyisedIn -->

    <owl:ObjectProperty rdf:about="https://w3id.org/polifonia/ontology/music-representation/isAnalyisedIn">
        <rdfs:subPropertyOf>
            <rdf:Description>
                <owl:inverseOf rdf:resource="http://linkedu.eu/dedalo/explanationPattern.owl#hasExplanandum"/>
            </rdf:Description>
        </rdfs:subPropertyOf>
        <rdf:type rdf:resource="http://www.w3.org/2002/07/owl#InverseFunctionalProperty"/>
        <rdfs:domain rdf:resource="https://w3id.org/polifonia/ontology/music-representation/MusicContent"/>
        <rdfs:range rdf:resource="https://w3id.org/polifonia/ontology/music-representation/Analysis"/>
        <rdfs:comment xml:lang="en">The relantionship that identifies an analysis of a specific music content.</rdfs:comment>
        <rdfs:label xml:lang="en">is analysed in</rdfs:label>
    </owl:ObjectProperty>
    


    <!-- https://w3id.org/polifonia/ontology/music-representation/isAnnotatedIn -->

    <owl:ObjectProperty rdf:about="https://w3id.org/polifonia/ontology/music-representation/isAnnotatedIn">
        <rdfs:subPropertyOf rdf:resource="http://www.ontologydesignpatterns.org/cp/owl/descriptionandsituation.owl#describes"/>
        <rdfs:domain rdf:resource="https://w3id.org/polifonia/ontology/music-representation/Analysis"/>
        <rdfs:domain rdf:resource="https://w3id.org/polifonia/ontology/music-representation/MusicContent"/>
        <rdfs:range rdf:resource="https://w3id.org/polifonia/ontology/music-representation/Annotation"/>
        <rdfs:comment xml:lang="en">A direct relationship between a music content and an annotation. Some specific content (e.g. elements of a score) might be annotated without the need of an analysis.</rdfs:comment>
        <rdfs:label xml:lang="en">is annotated in</rdfs:label>
    </owl:ObjectProperty>
    


    <!-- https://w3id.org/polifonia/ontology/music-representation/isBasedOn -->

    <owl:ObjectProperty rdf:about="https://w3id.org/polifonia/ontology/music-representation/isBasedOn">
        <rdfs:subPropertyOf rdf:resource="http://linkedu.eu/dedalo/explanationPattern.owl#hasExplanans"/>
        <rdfs:domain rdf:resource="https://w3id.org/polifonia/ontology/music-representation/Analysis"/>
        <rdfs:range rdf:resource="https://w3id.org/polifonia/ontology/music-representation/AnalyticalReference"/>
        <rdfs:comment xml:lang="en">Relationship between an analysis and its analytical reference.</rdfs:comment>
        <rdfs:label xml:lang="en">is based on</rdfs:label>
    </owl:ObjectProperty>
    


    <!-- https://w3id.org/polifonia/ontology/music-representation/isComposedOf -->

    <owl:ObjectProperty rdf:about="https://w3id.org/polifonia/ontology/music-representation/isComposedOf">
        <rdfs:subPropertyOf rdf:resource="http://www.ontologydesignpatterns.org/cp/owl/partof.owl#hasPart"/>
        <rdfs:domain rdf:resource="https://w3id.org/polifonia/ontology/music-representation/MusicNotation"/>
        <rdfs:range rdf:resource="https://w3id.org/polifonia/ontology/music-representation/MusicNotation"/>
        <rdfs:comment xml:lang="en">Part-of relationship between two music notation entities. 
E.g. a chord is composed of pitchclasses.</rdfs:comment>
        <rdfs:label xml:lang="en">is composed of</rdfs:label>
    </owl:ObjectProperty>
    


    <!-- 
    ///////////////////////////////////////////////////////////////////////////////////////
    //
    // Data properties
    //
    ///////////////////////////////////////////////////////////////////////////////////////
     -->

    


    <!-- https://w3id.org/polifonia/ontology/music-representation/hasConfidence -->

    <owl:DatatypeProperty rdf:about="https://w3id.org/polifonia/ontology/music-representation/hasConfidence">
        <rdfs:domain rdf:resource="https://w3id.org/polifonia/ontology/music-representation/Analysis"/>
        <rdfs:range rdf:resource="http://www.w3.org/2000/01/rdf-schema#Literal"/>
        <rdfs:comment xml:lang="en">The confidence of an analysis.</rdfs:comment>
        <rdfs:label xml:lang="en">has confidence</rdfs:label>
    </owl:DatatypeProperty>
    


    <!-- 
    ///////////////////////////////////////////////////////////////////////////////////////
    //
    // Classes
    //
    ///////////////////////////////////////////////////////////////////////////////////////
     -->

    


    <!-- http://linkeddata.uni-muenster.de/ontology/musicscore#Accidental -->

    <rdf:Description rdf:about="http://linkeddata.uni-muenster.de/ontology/musicscore#Accidental">
        <rdfs:subClassOf rdf:resource="https://w3id.org/polifonia/ontology/music-representation/MusicNotation"/>
    </rdf:Description>
    


    <!-- http://linkeddata.uni-muenster.de/ontology/musicscore#Articulation -->

    <rdf:Description rdf:about="http://linkeddata.uni-muenster.de/ontology/musicscore#Articulation">
        <rdfs:subClassOf rdf:resource="https://w3id.org/polifonia/ontology/music-representation/MusicNotation"/>
    </rdf:Description>
    


    <!-- http://linkeddata.uni-muenster.de/ontology/musicscore#Clef -->

    <rdf:Description rdf:about="http://linkeddata.uni-muenster.de/ontology/musicscore#Clef">
        <rdfs:subClassOf rdf:resource="https://w3id.org/polifonia/ontology/music-representation/MusicNotation"/>
    </rdf:Description>
    


    <!-- http://linkeddata.uni-muenster.de/ontology/musicscore#Duration -->

    <rdf:Description rdf:about="http://linkeddata.uni-muenster.de/ontology/musicscore#Duration">
        <rdfs:subClassOf rdf:resource="https://w3id.org/polifonia/ontology/music-representation/MusicNotation"/>
    </rdf:Description>
    


    <!-- http://linkeddata.uni-muenster.de/ontology/musicscore#DurationAttribute -->

    <rdf:Description rdf:about="http://linkeddata.uni-muenster.de/ontology/musicscore#DurationAttribute">
        <rdfs:subClassOf rdf:resource="https://w3id.org/polifonia/ontology/music-representation/MusicNotation"/>
    </rdf:Description>
    


    <!-- http://linkeddata.uni-muenster.de/ontology/musicscore#Dynamic -->

    <rdf:Description rdf:about="http://linkeddata.uni-muenster.de/ontology/musicscore#Dynamic">
        <rdfs:subClassOf rdf:resource="https://w3id.org/polifonia/ontology/music-representation/MusicNotation"/>
    </rdf:Description>
    


    <!-- http://linkeddata.uni-muenster.de/ontology/musicscore#Instant -->

    <rdf:Description rdf:about="http://linkeddata.uni-muenster.de/ontology/musicscore#Instant">
        <rdfs:subClassOf rdf:resource="https://w3id.org/polifonia/ontology/music-representation/Fragment"/>
    </rdf:Description>
    


    <!-- http://linkeddata.uni-muenster.de/ontology/musicscore#InterpretationMarking -->

    <rdf:Description rdf:about="http://linkeddata.uni-muenster.de/ontology/musicscore#InterpretationMarking">
        <rdfs:subClassOf rdf:resource="https://w3id.org/polifonia/ontology/music-representation/MusicNotation"/>
    </rdf:Description>
    


    <!-- http://linkeddata.uni-muenster.de/ontology/musicscore#Measure -->

    <rdf:Description rdf:about="http://linkeddata.uni-muenster.de/ontology/musicscore#Measure">
        <rdfs:subClassOf rdf:resource="https://w3id.org/polifonia/ontology/music-representation/MusicNotation"/>
    </rdf:Description>
    


    <!-- http://linkeddata.uni-muenster.de/ontology/musicscore#NoteAttribute -->

    <rdf:Description rdf:about="http://linkeddata.uni-muenster.de/ontology/musicscore#NoteAttribute">
        <rdfs:subClassOf rdf:resource="https://w3id.org/polifonia/ontology/music-representation/MusicNotation"/>
    </rdf:Description>
    


    <!-- http://linkeddata.uni-muenster.de/ontology/musicscore#NoteLink -->

    <rdf:Description rdf:about="http://linkeddata.uni-muenster.de/ontology/musicscore#NoteLink">
        <rdfs:subClassOf rdf:resource="https://w3id.org/polifonia/ontology/music-representation/MusicNotation"/>
    </rdf:Description>
    


    <!-- http://linkeddata.uni-muenster.de/ontology/musicscore#NoteSet -->

    <rdf:Description rdf:about="http://linkeddata.uni-muenster.de/ontology/musicscore#NoteSet">
        <rdfs:subClassOf rdf:resource="https://w3id.org/polifonia/ontology/music-representation/MusicNotation"/>
    </rdf:Description>
    


    <!-- http://linkeddata.uni-muenster.de/ontology/musicscore#Repeat -->

    <rdf:Description rdf:about="http://linkeddata.uni-muenster.de/ontology/musicscore#Repeat">
        <rdfs:subClassOf rdf:resource="https://w3id.org/polifonia/ontology/music-representation/MusicNotation"/>
    </rdf:Description>
    


    <!-- http://linkeddata.uni-muenster.de/ontology/musicscore#Staff -->

    <rdf:Description rdf:about="http://linkeddata.uni-muenster.de/ontology/musicscore#Staff">
        <rdfs:subClassOf rdf:resource="https://w3id.org/polifonia/ontology/music-representation/MusicNotation"/>
    </rdf:Description>
    


    <!-- http://linkeddata.uni-muenster.de/ontology/musicscore#TempoMarking -->

    <rdf:Description rdf:about="http://linkeddata.uni-muenster.de/ontology/musicscore#TempoMarking">
        <rdfs:subClassOf rdf:resource="https://w3id.org/polifonia/ontology/music-representation/MusicNotation"/>
    </rdf:Description>
    


    <!-- http://linkeddata.uni-muenster.de/ontology/musicscore#TimeSignature -->

    <rdf:Description rdf:about="http://linkeddata.uni-muenster.de/ontology/musicscore#TimeSignature">
        <rdfs:subClassOf rdf:resource="https://w3id.org/polifonia/ontology/music-representation/MusicNotation"/>
    </rdf:Description>
    


    <!-- http://linkeddata.uni-muenster.de/ontology/musicscore#Tuplet -->

    <rdf:Description rdf:about="http://linkeddata.uni-muenster.de/ontology/musicscore#Tuplet">
        <rdfs:subClassOf rdf:resource="https://w3id.org/polifonia/ontology/music-representation/MusicNotation"/>
    </rdf:Description>
    


    <!-- http://linkeddata.uni-muenster.de/ontology/musicscore#Voice -->

    <rdf:Description rdf:about="http://linkeddata.uni-muenster.de/ontology/musicscore#Voice">
        <rdfs:subClassOf rdf:resource="https://w3id.org/polifonia/ontology/music-representation/MusicNotation"/>
    </rdf:Description>
    


    <!-- https://w3id.org/polifonia/ontology/music-representation/Analysis -->

    <owl:Class rdf:about="https://w3id.org/polifonia/ontology/music-representation/Analysis">
        <rdfs:subClassOf>
            <owl:Restriction>
                <owl:onProperty rdf:resource="https://w3id.org/polifonia/ontology/music-representation/isBasedOn"/>
                <owl:allValuesFrom rdf:resource="https://w3id.org/polifonia/ontology/music-representation/AnalyticalReference"/>
            </owl:Restriction>
        </rdfs:subClassOf>
        <rdfs:subClassOf>
            <owl:Restriction>
                <owl:onProperty rdf:resource="https://w3id.org/polifonia/ontology/music-representation/hasConfidence"/>
                <owl:someValuesFrom rdf:resource="http://www.w3.org/2000/01/rdf-schema#Literal"/>
            </owl:Restriction>
        </rdfs:subClassOf>
        <rdfs:comment xml:lang="en">As defined by Marsden in &quot;Music Analysis by Computer: Ontology and
Epistemology&quot;, an analysis is a process that adds information to a musical piece in the sense that someone reading an analysis will gain knowledge that they did not have before.
It never adds anything to a musical piece that was not implicitly in it.

For example, an analysis that classifies a piece in &quot;Sonata Form&quot; does not simply provide a label for a piece but rather provides specific analytical evidences that justify the classification.</rdfs:comment>
        <rdfs:label xml:lang="en">Analysis</rdfs:label>
    </owl:Class>
    


    <!-- https://w3id.org/polifonia/ontology/music-representation/AnalyticalReference -->

    <owl:Class rdf:about="https://w3id.org/polifonia/ontology/music-representation/AnalyticalReference">
        <rdfs:comment xml:lang="en">An analytical reference is a musical theory, i.e. a set of assumptions and commitments that an analyst make when producing an analysis. The result of an analysis is ultimately one of the possible interpretation of a musical piece: different theories can result in the same result as well as same theories can be used to obtain different results.

An example is Riemann&apos;s theory or Schenker&apos;s theory.</rdfs:comment>
        <rdfs:label xml:lang="en">Analytical reference</rdfs:label>
    </owl:Class>
    


    <!-- https://w3id.org/polifonia/ontology/music-representation/Annotation -->

    <owl:Class rdf:about="https://w3id.org/polifonia/ontology/music-representation/Annotation">
        <rdfs:subClassOf>
            <owl:Class>
                <owl:unionOf rdf:parseType="Collection">
                    <owl:Restriction>
                        <owl:onProperty>
                            <rdf:Description>
                                <owl:inverseOf rdf:resource="https://w3id.org/polifonia/ontology/music-representation/isAnnotatedIn"/>
                            </rdf:Description>
                        </owl:onProperty>
                        <owl:someValuesFrom rdf:resource="https://w3id.org/polifonia/ontology/music-representation/Analysis"/>
                    </owl:Restriction>
                    <owl:Restriction>
                        <owl:onProperty>
                            <rdf:Description>
                                <owl:inverseOf rdf:resource="https://w3id.org/polifonia/ontology/music-representation/isAnnotatedIn"/>
                            </rdf:Description>
                        </owl:onProperty>
                        <owl:someValuesFrom rdf:resource="https://w3id.org/polifonia/ontology/music-representation/MusicContent"/>
                    </owl:Restriction>
                </owl:unionOf>
            </owl:Class>
        </rdfs:subClassOf>
        <rdfs:subClassOf>
            <owl:Restriction>
                <owl:onProperty rdf:resource="https://w3id.org/polifonia/ontology/music-representation/describes"/>
                <owl:someValuesFrom rdf:resource="https://w3id.org/polifonia/ontology/music-representation/Fragment"/>
            </owl:Restriction>
        </rdfs:subClassOf>
        <rdfs:subClassOf>
            <owl:Restriction>
                <owl:onProperty rdf:resource="https://w3id.org/polifonia/ontology/music-representation/hasAnnotationContent"/>
                <owl:someValuesFrom rdf:resource="https://w3id.org/polifonia/ontology/music-representation/AnnotationContent"/>
            </owl:Restriction>
        </rdfs:subClassOf>
        <rdfs:subClassOf>
            <owl:Restriction>
                <owl:onProperty rdf:resource="https://w3id.org/polifonia/ontology/music-representation/hasAnnotationType"/>
                <owl:someValuesFrom rdf:resource="https://w3id.org/polifonia/ontology/music-representation/AnnotationType"/>
            </owl:Restriction>
        </rdfs:subClassOf>
        <rdfs:subClassOf>
            <owl:Restriction>
                <owl:onProperty rdf:resource="https://w3id.org/polifonia/ontology/music-representation/derivesFrom"/>
                <owl:allValuesFrom rdf:resource="https://w3id.org/polifonia/ontology/music-representation/Annotation"/>
            </owl:Restriction>
        </rdfs:subClassOf>
        <rdfs:subClassOf>
            <owl:Restriction>
                <owl:onProperty rdf:resource="https://w3id.org/polifonia/ontology/music-representation/hasAnnotationType"/>
                <owl:allValuesFrom rdf:resource="https://w3id.org/polifonia/ontology/music-representation/AnnotationType"/>
            </owl:Restriction>
        </rdfs:subClassOf>
        <rdfs:subClassOf>
            <owl:Restriction>
                <owl:onProperty rdf:resource="https://w3id.org/polifonia/ontology/music-representation/hasAnnotator"/>
                <owl:allValuesFrom rdf:resource="https://w3id.org/polifonia/ontology/core/Agent"/>
            </owl:Restriction>
        </rdfs:subClassOf>
        <rdfs:subClassOf>
            <owl:Restriction>
                <owl:onProperty rdf:resource="https://w3id.org/polifonia/ontology/music-representation/hasAnnotationContent"/>
                <owl:minQualifiedCardinality rdf:datatype="http://www.w3.org/2001/XMLSchema#nonNegativeInteger">1</owl:minQualifiedCardinality>
                <owl:onClass rdf:resource="https://w3id.org/polifonia/ontology/music-representation/AnnotationContent"/>
            </owl:Restriction>
        </rdfs:subClassOf>
        <rdfs:subClassOf>
            <owl:Restriction>
                <owl:onProperty rdf:resource="https://w3id.org/polifonia/ontology/music-representation/hasAnnotationContent"/>
                <owl:maxQualifiedCardinality rdf:datatype="http://www.w3.org/2001/XMLSchema#nonNegativeInteger">1</owl:maxQualifiedCardinality>
                <owl:onClass rdf:resource="https://w3id.org/polifonia/ontology/music-representation/AnnotationContent"/>
            </owl:Restriction>
        </rdfs:subClassOf>
        <rdfs:comment xml:lang="en">An annotation is a temporal precise and unique observation that an agent makes when performing an analysis on a musical piece. It can either describe an entire musical content or a specific fragment of a musical content. The subject of an annotation is the projection of a specific music content.</rdfs:comment>
        <rdfs:label xml:lang="en">Annotation</rdfs:label>
    </owl:Class>
    


    <!-- https://w3id.org/polifonia/ontology/music-representation/AnnotationContent -->

    <owl:Class rdf:about="https://w3id.org/polifonia/ontology/music-representation/AnnotationContent">
        <rdfs:subClassOf>
            <owl:Restriction>
                <owl:onProperty rdf:resource="https://w3id.org/polifonia/ontology/music-representation/hasSubject"/>
                <owl:someValuesFrom rdf:resource="https://w3id.org/polifonia/ontology/music-representation/MusicNotation"/>
            </owl:Restriction>
        </rdfs:subClassOf>
        <rdfs:subClassOf>
            <owl:Restriction>
                <owl:onProperty rdf:resource="https://w3id.org/polifonia/ontology/music-representation/hasSubject"/>
                <owl:minQualifiedCardinality rdf:datatype="http://www.w3.org/2001/XMLSchema#nonNegativeInteger">1</owl:minQualifiedCardinality>
                <owl:onClass rdf:resource="https://w3id.org/polifonia/ontology/music-representation/MusicNotation"/>
            </owl:Restriction>
        </rdfs:subClassOf>
        <rdfs:comment xml:lang="en">The content of an annotation is the projection of the musical content it is describing.</rdfs:comment>
        <rdfs:label xml:lang="en">Annotation content</rdfs:label>
    </owl:Class>
    


    <!-- https://w3id.org/polifonia/ontology/music-representation/AnnotationType -->

    <owl:Class rdf:about="https://w3id.org/polifonia/ontology/music-representation/AnnotationType">
        <rdfs:comment xml:lang="en">The type of an annotation, such as &quot;textual&quot; or &quot;JAMS observation&quot;.</rdfs:comment>
        <rdfs:label xml:lang="en">Annotation type</rdfs:label>
    </owl:Class>
    


    <!-- https://w3id.org/polifonia/ontology/music-representation/AnnotatorType -->

    <owl:Class rdf:about="https://w3id.org/polifonia/ontology/music-representation/AnnotatorType">
        <rdfs:comment xml:lang="en">Type of an annotator, such as crowd collected, algorithmically derived, provided by an expert etc.</rdfs:comment>
        <rdfs:label xml:lang="en">Annotator type</rdfs:label>
    </owl:Class>
    


    <!-- https://w3id.org/polifonia/ontology/music-representation/AudioFeatures -->

    <owl:Class rdf:about="https://w3id.org/polifonia/ontology/music-representation/AudioFeatures"/>
    


    <!-- https://w3id.org/polifonia/ontology/music-representation/Fragment -->

    <owl:Class rdf:about="https://w3id.org/polifonia/ontology/music-representation/Fragment">
        <rdfs:subClassOf>
            <owl:Restriction>
                <owl:onProperty>
                    <rdf:Description>
                        <owl:inverseOf rdf:resource="https://w3id.org/polifonia/ontology/music-representation/hasFragment"/>
                    </rdf:Description>
                </owl:onProperty>
                <owl:someValuesFrom rdf:resource="https://w3id.org/polifonia/ontology/music-representation/MusicContent"/>
            </owl:Restriction>
        </rdfs:subClassOf>
        <rdfs:comment xml:lang="en">A fragment is the atomic piece that compose the final analysis. For example, when describing harmonic progression a fragment is the instant where a chord is played. When describing forms, a fragment is a section of a piece that spans several instants.</rdfs:comment>
        <rdfs:label xml:lang="en">Fragment</rdfs:label>
    </owl:Class>
    


    <!-- https://w3id.org/polifonia/ontology/music-representation/MusicContent -->

    <owl:Class rdf:about="https://w3id.org/polifonia/ontology/music-representation/MusicContent">
        <rdfs:subClassOf>
            <owl:Restriction>
                <owl:onProperty rdf:resource="https://w3id.org/polifonia/ontology/music-representation/hasFragment"/>
                <owl:allValuesFrom rdf:resource="https://w3id.org/polifonia/ontology/music-representation/Fragment"/>
            </owl:Restriction>
        </rdfs:subClassOf>
        <rdfs:subClassOf>
            <owl:Restriction>
                <owl:onProperty rdf:resource="https://w3id.org/polifonia/ontology/music-representation/isAnalyisedIn"/>
                <owl:allValuesFrom rdf:resource="https://w3id.org/polifonia/ontology/music-representation/Analysis"/>
            </owl:Restriction>
        </rdfs:subClassOf>
        <rdfs:subClassOf>
            <owl:Restriction>
                <owl:onProperty rdf:resource="https://w3id.org/polifonia/ontology/music-representation/isAnnotatedIn"/>
                <owl:allValuesFrom rdf:resource="https://w3id.org/polifonia/ontology/music-representation/Annotation"/>
            </owl:Restriction>
        </rdfs:subClassOf>
        <owl:disjointUnionOf rdf:parseType="Collection">
            <rdf:Description rdf:about="https://w3id.org/polifonia/ontology/music-meta/AbstractScore"/>
            <rdf:Description rdf:about="https://w3id.org/polifonia/ontology/music-meta/Score"/>
            <rdf:Description rdf:about="https://w3id.org/polifonia/ontology/music-representation/AudioFeatures"/>
        </owl:disjointUnionOf>
        <rdfs:comment xml:lang="en">Music content represents a musical piece that can be analysed by means of an analytical process.</rdfs:comment>
        <rdfs:label xml:lang="en">Music content</rdfs:label>
    </owl:Class>
    


    <!-- https://w3id.org/polifonia/ontology/music-representation/MusicNotation -->

    <owl:Class rdf:about="https://w3id.org/polifonia/ontology/music-representation/MusicNotation">
        <rdfs:subClassOf>
            <owl:Restriction>
                <owl:onProperty rdf:resource="https://w3id.org/polifonia/ontology/music-representation/isComposedOf"/>
                <owl:allValuesFrom rdf:resource="https://w3id.org/polifonia/ontology/music-representation/MusicNotation"/>
            </owl:Restriction>
        </rdfs:subClassOf>
        <rdfs:comment xml:lang="en">Music notation is the subject of an annotation content.

For example an music notation is a chord or a note.</rdfs:comment>
        <rdfs:label xml:lang="en">Music notation</rdfs:label>
    </owl:Class>
    


    <!-- 
    ///////////////////////////////////////////////////////////////////////////////////////
    //
    // Individuals
    //
    ///////////////////////////////////////////////////////////////////////////////////////
     -->

    


    <!-- http://linkeddata.uni-muenster.de/ontology/musicscore#Score -->

    <owl:NamedIndividual rdf:about="http://linkeddata.uni-muenster.de/ontology/musicscore#Score"/>
    


    <!-- http://linkeddata.uni-muenster.de/ontology/musicscore#ScorePart -->

    <owl:NamedIndividual rdf:about="http://linkeddata.uni-muenster.de/ontology/musicscore#ScorePart"/>
    


    <!-- https://w3id.org/polifonia/ontology/music-meta/Score -->

    <owl:NamedIndividual rdf:about="https://w3id.org/polifonia/ontology/music-meta/Score">
        <skos:relatedMatch rdf:resource="http://linkeddata.uni-muenster.de/ontology/musicscore#Score"/>
    </owl:NamedIndividual>
    


    <!-- https://w3id.org/polifonia/ontology/music-meta/ScorePart -->

    <owl:NamedIndividual rdf:about="https://w3id.org/polifonia/ontology/music-meta/ScorePart">
        <skos:relatedMatch rdf:resource="http://linkeddata.uni-muenster.de/ontology/musicscore#ScorePart"/>
    </owl:NamedIndividual>
    


    <!-- https://w3id.org/polifonia/ontology/music-representation/ComputerAlgorithm -->

    <owl:NamedIndividual rdf:about="https://w3id.org/polifonia/ontology/music-representation/ComputerAlgorithm">
        <rdf:type rdf:resource="https://w3id.org/polifonia/ontology/music-representation/AnnotatorType"/>
    </owl:NamedIndividual>
    


    <!-- https://w3id.org/polifonia/ontology/music-representation/Crowd -->

    <owl:NamedIndividual rdf:about="https://w3id.org/polifonia/ontology/music-representation/Crowd">
        <rdf:type rdf:resource="https://w3id.org/polifonia/ontology/music-representation/AnnotatorType"/>
    </owl:NamedIndividual>
    


    <!-- https://w3id.org/polifonia/ontology/music-representation/ExpertAnnotator -->

    <owl:NamedIndividual rdf:about="https://w3id.org/polifonia/ontology/music-representation/ExpertAnnotator">
        <rdf:type rdf:resource="https://w3id.org/polifonia/ontology/music-representation/AnnotatorType"/>
    </owl:NamedIndividual>
</rdf:RDF>



<!-- Generated by the OWL API (version 4.5.9.2019-02-01T07:24:44Z) https://github.com/owlcs/owlapi -->

